Issue state, error in `Barrier` file

src/examples/matmul-opt/GPU.MatMulOpt.Barrier.fsti
@@ -2,88 +2,160 @@ module GPU.MatMulOpt.Barrier
 
 #lang-pulse
 
+// #push-options "--log_queries"
+
 open GPU
 open GPU.Barrier.RPM
+open GPU.MatMulOpt.Array
+open GPU.MatMulOpt.Layout
 module Pure = GPU.MatMulOpt.Pure
 module SZ = FStar.SizeT
 
-#push-options "--admit_smt_queries true"
+#push-options "--fuel 8 --ifuel 8"
+
+let lemma_pos (x: pos): Lemma (0 < x * x) [SMTPat (x * x)] = ()
+
 let barrier_mm_share
-    (n: nat)
-    (s1 s2: seq (seq u64))
-    (ar: gpu_array u64 (2 * n))
-    (it: nat { it < Seq.length s1 /\ it < Seq.length s2 })
-    (from: nat { 0 <= from /\ from < n })
-    (to: nat { 0 <= to /\ to < n })
+    (#bdim #bdim_shared #bdim_cols #bdim_rows: pos)
+    (s1: mseq seq![bdim; bdim_shared; bdim; bdim_rows] u64)
+    (ar1: gpu_matrix u64 seq![bdim; bdim])
+    (s2: mseq seq![bdim; bdim_cols; bdim; bdim_shared] u64)
+    (ar2: gpu_matrix u64 seq![bdim; bdim])
+    (#bid_x: nat { 0 <= bid_x /\ bid_x < bdim_cols })
+    (#bid_y: nat { 0 <= bid_y /\ bid_y < bdim_rows })
+    (it: nat { 0 <= it /\ it < bdim_shared })
+    (from_x: nat { 0 <= from_x /\ from_x < bdim })
+    (from_y: nat { 0 <= from_y /\ from_y < bdim })
     : slprop
 =
-  gpu_pts_to_array_slice ar #(1.0R /. Real.of_int n)
-    from (from + 1) (Pure.singleton (Seq.index (Seq.index s1 it) from)) **
-  gpu_pts_to_array_slice ar #(1.0R /. Real.of_int n)
-    (from + n) (from + n + 1) (Pure.singleton (Seq.index (Seq.index s2 it) from))
-#pop-options
+  gpu_pts_to_matrix #u64 #seq![] (slice_matrix (slice_matrix ar1 1 from_y) 0 from_x) #(1.0R /. Real.of_int (bdim * bdim)) (Pure.singleton (index s1 seq![from_x; it; from_y; bid_y])) **
+  gpu_pts_to_matrix #u64 #seq![] (slice_matrix (slice_matrix ar2 1 from_y) 0 from_x) #(1.0R /. Real.of_int (bdim * bdim)) (Pure.singleton (index s2 seq![from_x; bid_x; from_y; it]))
 
 let barrier_mm_gather
-    (n: nat)
-    (ar: gpu_array u64 (2 * n))
-    (it: nat)
-    (from: nat { 0 <= from /\ from < n })
-    (to: nat { 0 <= to /\ to < n })
-    : slprop
-= bigstar 0 n (fun i -> cond (i = to) (gpu_pts_to_array1 ar #(1.0R /. Real.of_int n) i ** gpu_pts_to_array1 ar #(1.0R /. Real.of_int n) (i + n)) emp)
-
-let barrier_mm
-    (n: nat)
-    (s1 s2: seq (seq u64)) //  { Seq.length i == n }))
-    (ar: gpu_array u64 (2 * n))
-    (it: nat)
-    (from: nat { 0 <= from /\ from < n })
-    (to: nat { 0 <= to /\ to < n })
+    (#bdim #bdim_shared #bdim_cols #bdim_rows: pos)
+    (s1: mseq seq![bdim; bdim_shared; bdim; bdim_rows] u64)
+    (ar1: gpu_matrix u64 seq![bdim; bdim])
+    (s2: mseq seq![bdim; bdim_cols; bdim; bdim_shared] u64)
+    (ar2: gpu_matrix u64 seq![bdim; bdim])
+    (#bid_x: nat { 0 <= bid_x /\ bid_x < bdim_cols })
+    (#bid_y: nat { 0 <= bid_y /\ bid_y < bdim_rows })
+    (it: nat { 0 <= it /\ it < bdim_shared })
+    (to_x: nat { 0 <= to_x /\ to_x < bdim })
+    (to_y: nat { 0 <= to_y /\ to_y < bdim })
     : slprop
 =
-  if (it / 2 < Seq.length s1 && it / 2 < Seq.length s2)
-  then (cond (it % 2 = 0) (barrier_mm_share n s1 s2 ar (it / 2) from to) (barrier_mm_gather n ar (it / 2) from to))
-  else emp
+  gpu_pts_to_matrix #u64 #seq![] (slice_matrix (slice_matrix ar1 1 to_y) 0 to_x) #(1.0R /. Real.of_int (bdim * bdim)) (Pure.singleton (index s1 seq![to_x; it; to_y; bid_y])) **
+  gpu_pts_to_matrix #u64 #seq![] (slice_matrix (slice_matrix ar2 1 to_y) 0 to_x) #(1.0R /. Real.of_int (bdim * bdim)) (Pure.singleton (index s2 seq![to_x; bid_x; to_y; it]))
 
-let shared_pre (nthr : sz { 0 < nthr /\ nthr <= max_threads })
-    (s1 s2: seq (seq u64))
-    (it: nat) (ar: gpu_array u64 SZ.(2sz *^ nthr)) (i: nat { 0 <= i /\ i < nthr })
+let multiply_2_lemma (a b: pos): Lemma (multiply seq![a; b] = a * b) [SMTPat (seq![a; b])] = ()
+let multiply_3_lemma (a b c: pos): Lemma (multiply seq![a; b; c] = a * b * c) [SMTPat (seq![a; b; c])] = ()
+
+let barrier_mm
+    (#bdim #bdim_shared #bdim_cols #bdim_rows: pos)
+    (s1: mseq seq![bdim; bdim_shared; bdim; bdim_rows] u64)
+    (ar1: gpu_matrix u64 seq![bdim; bdim])
+    (s2: mseq seq![bdim; bdim_cols; bdim; bdim_shared] u64)
+    (ar2: gpu_matrix u64 seq![bdim; bdim])
+    (bid_x: nat { 0 <= bid_x /\ bid_x < bdim_cols })
+    (bid_y: nat { 0 <= bid_y /\ bid_y < bdim_rows })
+    (it: nat)
+    (from: nat { 0 <= from /\ from < bdim * bdim })
+    (to: nat { 0 <= to /\ to < bdim * bdim })
+    : slprop
+= 
+  let from_split = split_to_dims seq![bdim; bdim] from in
+  let to_split = split_to_dims seq![bdim; bdim] to in
+    if (it / 2 < bdim_shared)
+    then (cond (it % 2 = 0) (barrier_mm_share s1 ar1 s2 ar2 #bid_x #bid_y (it / 2) from_split.[0] from_split.[1])
+                            (barrier_mm_gather s1 ar1 s2 ar2 #bid_x #bid_y (it / 2) to_split.[0] to_split.[1]))
+    else emp
+
+let shared_pre
+    (#bdim #bdim_shared #bdim_cols #bdim_rows: pos)
+    (s1: mseq seq![bdim; bdim_shared; bdim; bdim_rows] u64)
+    (ar1: gpu_matrix u64 seq![bdim; bdim])
+    (s2: mseq seq![bdim; bdim_cols; bdim; bdim_shared] u64)
+    (ar2: gpu_matrix u64 seq![bdim; bdim])
+    (bid_x: nat { 0 <= bid_x /\ bid_x < bdim_cols })
+    (bid_y: nat { 0 <= bid_y /\ bid_y < bdim_rows })
+    (it: nat)
+    (i: nat { 0 <= i /\ i < bdim * bdim })
 : slprop
-= gpu_pts_to_array1 ar i **
-  gpu_pts_to_array1 ar (i + nthr) ** mbarrier_tok nthr (barrier_mm nthr s1 s2 ar) it i
+=
+  let i_split = split_to_dims seq![bdim; bdim] i in
+  gpu_pts_to_matrix #u64 #seq![] (slice_matrix (slice_matrix ar1 1 i_split.[1]) 0 i_split.[0]) #1.0R (Pure.singleton 0uL) **
+  gpu_pts_to_matrix #u64 #seq![] (slice_matrix (slice_matrix ar2 1 i_split.[1]) 0 i_split.[0]) #1.0R (Pure.singleton 0uL) **
+  mbarrier_tok (bdim * bdim) (barrier_mm s1 ar1 s2 ar2 bid_x bid_y) it i
+
+
+// let gpu_matrix (a:Type u#0) (dims: FStar.Seq.seq pos) : Type u#0 = gpu_array a (multiply dims)
+let to_gpu_matrix (#a:Type u#0) (dims: FStar.Seq.seq pos) (ar: gpu_array a (multiply dims)): gpu_matrix a dims = ar
+
+val mk_gpu_array (a:Type u#0) (dims: FStar.Seq.seq pos): gpu_matrix a dims
+
+let remove_lemma #a (x y z: a): Lemma (remove seq![x; y; z] 0 == seq![y; z])// [SMTPat (remove seq![x; y; z] 0)]
+  = FStar.Seq.lemma_eq_intro (remove seq![x; y; z] 0) seq![y; z]
+
+// #set-options "--debug SMTFail --split_queries always"
 
 ghost
 fn block_setup_ghost
-  (nblk : sz { 0 < reveal nblk /\ reveal nblk <= max_blocks })
-  (nthr : sz { 0 < nthr /\ nthr <= max_threads })
-  (smem_sz : sz { smem_sz == SZ.(2sz *^ nthr) })
+  (#bdim #bdim_shared #bdim_cols #bdim_rows: pos)
+  (s1: mseq seq![bdim; bdim_shared; bdim; bdim_rows] u64)
+  // (ar1: gpu_matrix u64 seq![bdim; bdim])
+  (s2: mseq seq![bdim; bdim_cols; bdim; bdim_shared] u64)
+  // (ar2: gpu_matrix u64 seq![bdim; bdim])
+  (nblk : sz { 0 < nblk /\ nblk <= max_blocks /\ SZ.v nblk == bdim_cols * bdim_rows })
+  (nthr : sz { 0 < nthr /\ nthr <= max_threads /\ SZ.v nblk == bdim * bdim })
+  (smem_sz : sz { SZ.v smem_sz == 2 * bdim * bdim })
   (ar: gpu_array u64 smem_sz)
-  (bid: sz { 0 <= bid /\ SZ.v bid < SZ.v nblk })
+  (bid: sz { 0 <= bid /\ SZ.v bid < bdim_cols * bdim_rows })
   requires block_setup nthr ** (exists* v. gpu_pts_to_array #u64 #smem_sz ar #1.0R v)
-  ensures block_setup nthr ** bigstar 0 nthr (shared_pre nthr Seq.empty Seq.empty 0 ar)
+  ensures (let bid_split = split_to_dims seq![bdim_cols; bdim_rows] bid in
+           let ar_split = to_gpu_matrix seq![2 <: pos; bdim; bdim] ar in
+           (//remove_lemma (2 <: pos) bdim bdim; assert (remove seq![2 <: pos; bdim; bdim] 0 == seq![bdim; bdim]);
+          //  let ar1: gpu_matrix u64 seq![bdim; bdim] = slice_matrix ar_split 0 0 in
+          //  let ar2: gpu_matrix u64 seq![bdim; bdim] = slice_matrix ar_split 0 1 in
+    block_setup nthr ** bigstar 0 nblk (shared_pre s1 (mk_gpu_array u64 seq![bdim; bdim]) s2 (mk_gpu_array u64 seq![bdim; bdim]) bid_split.[0] bid_split.[1] 0)))
 {
-  with v. assert (gpu_pts_to_array #u64 #smem_sz ar #1.0R v);
-  unfold gpu_pts_to_array ar v;
-  gpu_slice_slice_1_underspec #1 ar #1.0R 0 smem_sz nthr;
-  drop_   (bigstar #1 0 (SZ.v nthr - 0) (fun x -> gpu_pts_to_array1 ar (x + 0)));
-  assume_ (bigstar #1 0 nthr            (fun x -> gpu_pts_to_array1 ar x));
+  // let dims_inner: seq pos = seq![bdim; bdim; 2 <: pos];
+  // let t: Type u#0 = (gpu_matrix u64 seq![bdim; bdim; 2] <: Type u#0);
 
-  gpu_slice_slice_1_underspec #2 ar #1.0R nthr smem_sz smem_sz;
-  drop_   (bigstar #2 0 (smem_sz - nthr) (fun x -> gpu_pts_to_array1 ar (x + nthr)));
-  assume_ (bigstar #2 0 nthr             (fun x -> gpu_pts_to_array1 ar (x + nthr)));
+  assert (pure (multiply seq![2 <: pos; bdim; bdim] == 2 * bdim * bdim));
+  let ar_split = (to_gpu_matrix seq![2 <: pos; bdim; bdim] ar) <: gpu_matrix u64 seq![2 <: pos; bdim; bdim];
+  FStar.Seq.lemma_eq_intro (remove seq![2 <: pos; bdim; bdim] 0) seq![bdim; bdim];
+  assert (pure (remove seq![2 <: pos; bdim; bdim] 0 == seq![bdim; bdim] /\ gpu_matrix u64 (remove seq![2 <: pos; bdim; bdim] 0) == gpu_matrix u64 seq![bdim; bdim]));
+  let ar1 = slice_matrix ar_split 0 0 <: gpu_matrix u64 (remove seq![2 <: pos; bdim; bdim] 0);
+  
+  let ar11 = (*coerce_eq ()*) ar1 <: gpu_matrix u64 seq![bdim; bdim];
+  admit();
+  ()
+  // with v. assert (gpu_pts_to_array #u64 #smem_sz ar #1.0R v);
+  // unfold gpu_pts_to_array ar v;
+  // gpu_slice_slice_1_underspec #1 ar #1.0R 0 smem_sz (bdim * bdim);
+  // drop_   (bigstar #1 0 (SZ.v nthr - 0) (fun x -> gpu_pts_to_array1 ar (x + 0)));
+  // assume_ (bigstar #1 0 nthr            (fun x -> gpu_pts_to_array1 ar x));
 
-  bigstar_zip #1 #2 #1 0 nthr _ _;
+  // gpu_slice_slice_1_underspec #2 ar #1.0R nthr smem_sz smem_sz;
+  // drop_   (bigstar #2 0 (smem_sz - nthr) (fun x -> gpu_pts_to_array1 ar (x + nthr)));
+  // assume_ (bigstar #2 0 nthr             (fun x -> gpu_pts_to_array1 ar (x + nthr)));
 
-  mk_mbarrier nthr (barrier_mm nthr Seq.empty Seq.empty ar);
-  bigstar_zip #1 #0 #0 0 nthr _ _;
+  // bigstar_zip #1 #2 #1 0 nthr _ _;
 
-  // FOLD:
-  drop_   (bigstar #0 0 nthr (fun x -> gpu_pts_to_array1 ar x ** gpu_pts_to_array1 ar (x + nthr) ** mbarrier_tok nthr (barrier_mm nthr Seq.empty Seq.empty ar) 0 x));
-  assume_ (bigstar #0 0 nthr (fun x -> shared_pre nthr Seq.empty Seq.empty 0 ar x));
+  // mk_mbarrier nthr (barrier_mm nthr Seq.empty Seq.empty ar);
+  // bigstar_zip #1 #0 #0 0 nthr _ _;
 
-  bigstar_uneta();
-  gpu_slice_empty_elim ar smem_sz;
+  // // FOLD:
+  // drop_   (bigstar #0 0 nthr (fun x -> gpu_pts_to_array1 ar x ** gpu_pts_to_array1 ar (x + nthr) ** mbarrier_tok nthr (barrier_mm nthr Seq.empty Seq.empty ar) 0 x));
+  // assume_ (bigstar #0 0 nthr (fun x -> shared_pre nthr Seq.empty Seq.empty 0 ar x));
+
+  // bigstar_uneta();
+  // gpu_slice_empty_elim ar smem_sz;
 }
 
-let shared_post (nthr : sz { 0 < nthr /\ nthr <= max_threads }) (ar: gpu_array u64 SZ.(2sz *^ nthr)) (i: nat { 0 <= i /\ i < nthr }): slprop =
-  exists* it. shared_pre nthr Seq.empty Seq.empty it ar i
+// bdim_shared == shared / tdim_y
+// let split_input_a2 (shared: pos) (bidx_x: nat) (tdim_x bdim_x tdim_y bdim_shared: pos) (a2: seq u64 { FStar.Seq.length a2 == tdim_y * bdim_shared * tdim_x * bdim_x  }): seq (seq u64)
+//   = FStar.Seq.init bdim_shared (fun bidx_y -> FStar.Seq.init (tdim_x * tdim_y) (fun tidx -> ))
+
+// let shared_post (nthr : sz { 0 < nthr /\ nthr <= max_threads }) (ar: gpu_array u64 SZ.(2sz *^ nthr)) (i: nat { 0 <= i /\ i < nthr }): slprop =
+//   exists* it. shared_pre nthr Seq.empty Seq.empty it ar i
