src/examples/matmul-opt/GPU.MatMulOpt.Array.fsti
@@ -1,0 +1,71 @@
+module GPU.MatMulOpt.Array
+
+#push-options "--fuel 1 --ifuel 1"
+
+#lang-pulse
+
+open FStar.Tactics.V2
+open FStar.Mul
+open Pulse.Lib.Pervasives
+open GPU
+
+open GPU.MatMulOpt.Layout
+
+type mseq (dims: FStar.Seq.seq pos) (a: Type) = (s: FStar.Seq.seq a { FStar.Seq.length s == multiply dims })
+
+let init #a (dims: FStar.Seq.seq pos) (f: (idxs: FStar.Seq.seq nat { FStar.Seq.length idxs == FStar.Seq.length dims /\ elementwise_smaller idxs dims }) -> a): mseq dims a
+  = FStar.Seq.init (multiply dims) (fun i -> f (split_to_dims dims i))
+
+let index #dims #a (s: mseq dims a) (idx: FStar.Seq.seq nat { FStar.Seq.length dims == FStar.Seq.length idx /\ elementwise_smaller idx dims }): a
+  =  s.[join_from_dims dims idx]
+
+let remove #a (s: FStar.Seq.seq a) (idx: nat { idx < FStar.Seq.length s }): (r: FStar.Seq.seq a { FStar.Seq.length r == FStar.Seq.length s - 1 })
+  = FStar.Seq.init (FStar.Seq.length s - 1) (fun i -> if i < idx then s.[i] else s.[i + 1])
+
+let insert #a (s: FStar.Seq.seq a) (elem: a) (idx: nat { idx <= FStar.Seq.length s }): (r: FStar.Seq.seq a { FStar.Seq.length r == FStar.Seq.length s + 1 })
+  = FStar.Seq.init (FStar.Seq.length s + 1) (fun i -> if i < idx then s.[i] else if i = idx then elem else s.[i - 1])
+
+// TODO
+let lemma_ews_remove_insert (dims: FStar.Seq.seq pos) (dim: nat { dim < FStar.Seq.length dims }) (idx: nat { idx < dims.[dim] }) (i: nat { i < multiply (remove dims dim) }):
+  Lemma (elementwise_smaller (insert (split_to_dims (remove dims dim) i) idx dim) dims) = admit()
+
+let slice #dims #a (s: mseq dims a) (dim: nat { dim < FStar.Seq.length dims }) (idx: nat { idx < dims.[dim] }): mseq (remove dims dim) a
+  = let new_dims = remove dims dim in FStar.Seq.init (multiply new_dims) (fun i ->
+    let idxs = insert (split_to_dims new_dims i) idx dim in
+      lemma_ews_remove_insert dims dim idx i;
+      index s idxs
+  )
+
+let gpu_matrix (a:Type u#0) (dims: FStar.Seq.seq pos) : Type u#0 = gpu_array a (multiply dims)
+
+let gpu_pts_to_matrix
+  (#a: Type u#0)
+  (#dims: FStar.Seq.seq pos)
+  (x: gpu_matrix a dims)
+  (#[exact (`1.0R)] f : perm)
+  (v : mseq dims a)
+: slprop = gpu_pts_to_array x #f v
+
+val slice_matrix #a #dims (ga: gpu_matrix a dims) (dim: nat { dim < FStar.Seq.length dims }) (idx: nat { idx < dims.[dim] }): gpu_matrix a (remove dims dim)
+  // = ga + idx * multiply dims[..dim]
+
+fn gpu_matrix_read
+  #a
+  (#dims: FStar.Seq.seq pos)
+  (ga : gpu_matrix a dims)
+  (#s: erased (mseq dims a))
+  (idxs: FStar.Seq.seq nat { FStar.Seq.length dims == FStar.Seq.length idxs /\ elementwise_smaller idxs dims })
+  requires gpu ** gpu_pts_to_matrix ga #1.0R s
+  returns v: a
+  ensures gpu ** gpu_pts_to_matrix ga #1.0R s ** pure (v == index s idxs)
+
+ghost
+fn gpu_matrix_slice_permission
+  #a
+  (#dims: FStar.Seq.seq pos)
+  (ga : gpu_matrix a dims)
+  (#f : perm)
+  (#s: erased (mseq dims a))
+  (dim: nat { dim < FStar.Seq.length dims })
+  requires gpu ** gpu_pts_to_matrix ga #f s
+  ensures gpu ** bigstar 0 dims.[dim] (fun i -> gpu_pts_to_matrix (slice_matrix ga dim i) #f (slice s dim i))
